Add more kinding/typing rules

theories/typing.v
@@ -1,17 +1,27 @@
 From Coq Require Import List.
 Import ListNotations.
 
+Require Import stdpp.list.
+
 Require Import RecordUpdate.RecordUpdate.
 
 Require Import RichWasm.syntax.
 
+Definition local_context := list type.
+
 Record function_context :=
-  { fc_loc_vars : nat;
+  { fc_result_type : list type;
+    fc_labels : list (list type * local_context);
+    fc_location_vars : nat;
     fc_rep_vars : nat;
     fc_type_vars : list kind }.
 
 Global Instance eta_function_context : Settable _ :=
-  settable! Build_function_context <fc_loc_vars; fc_rep_vars; fc_type_vars>.
+  settable! Build_function_context
+  <fc_result_type; fc_labels; fc_location_vars; fc_rep_vars; fc_type_vars>.
+
+Definition update_locals (le : local_effect) (L : local_context) : local_context :=
+  fold_left (fun acc '(i, τ) => <[ i := τ ]> acc) le L.
 
 Inductive rep_ok : function_context -> representation -> Prop :=
 | VarR_OK (F : function_context) (ϱ : variable) :
@@ -51,6 +61,12 @@ Inductive has_mono_size : representation -> nat -> Prop :=
   has_mono_size (PrimR F64R) 2.
 
 Inductive has_kind : function_context -> type -> kind -> Prop :=
+| KSubLin (F : function_context) (τ : type) (r : representation) (h : heapability) :
+  has_kind F τ (TYPE r Unr h) ->
+  has_kind F τ (TYPE r Lin h)
+| KSubHeap (F : function_context) (τ : type) (r : representation) (l : linearity) :
+  has_kind F τ (TYPE r l Heapable) ->
+  has_kind F τ (TYPE r l Unheapable)
 | KVar (F : function_context) (α : variable) (κ : kind) :
   nth_error F.(fc_type_vars) α = Some κ ->
   kind_ok F κ ->
@@ -77,7 +93,7 @@ Inductive has_kind : function_context -> type -> kind -> Prop :=
   has_kind F τ (TYPE r Unr Heapable) ->
   has_kind F (ArrayT τ) (TYPE DynR Unr Heapable)
 | KExLoc (F : function_context) (τ : type) (κ : kind) :
-  has_kind (set fc_loc_vars S F) τ κ ->
+  has_kind (set fc_location_vars S F) τ κ ->
   has_kind F (ExT ELoc τ) κ
 | KExType (F : function_context) (τ : type) (κ0 κ : kind) :
   has_kind (set fc_type_vars (cons κ0) F) τ κ ->
@@ -106,3 +122,84 @@ Inductive has_kind : function_context -> type -> kind -> Prop :=
   has_kind F (RepT r τ) (TYPE r l h)
 | KSized (F : function_context) (r : representation) :
   has_kind F (SizedT r) (CONSTRAINT (PrimR I32R)).
+
+Inductive is_unrestricted : function_context -> type -> Prop :=
+| UnrTYPE (F : function_context) (τ : type) (r : representation) (h : heapability) :
+  has_kind F τ (TYPE r Unr h) ->
+  is_unrestricted F τ
+| UnrCONSTRAINT (F : function_context) (τ : type) (r : representation) :
+  has_kind F τ (CONSTRAINT r) ->
+  is_unrestricted F τ.
+
+(* TODO *)
+Inductive num_instr_has_type : num_instr -> arrow_type -> Prop :=.
+
+Inductive instr_has_type {A : Type} :
+  function_context -> local_context -> instr A -> arrow_type -> local_context -> Prop :=
+| TNop (F : function_context) (L : local_context) (ann : A) :
+  instr_has_type F L (INop ann) (ArrowT [] []) L
+| TDrop (F : function_context) (L : local_context) (ann : A) (τ : type) :
+  is_unrestricted F τ ->
+  instr_has_type F L (IDrop ann) (ArrowT [τ] []) L
+| TUnreachable
+    (F : function_context) (L L' : local_context) (ann : A) (τs1 τs2 : list type) (le : local_effect) :
+  L' = update_locals le L ->
+  instr_has_type F L (IUnreachable ann) (ArrowT τs1 τs2) L
+| TNum (F : function_context) (L : local_context) (ann : A) (en : num_instr) (τa : arrow_type) :
+  num_instr_has_type en τa ->
+  instr_has_type F L (INum ann en) τa L
+| TNumConst (F : function_context) (L : local_context) (ann : A) (τn : num_type) (n : nat) :
+  instr_has_type F L (INumConst ann τn n) (ArrowT [] [NumT τn]) L
+| TBlock
+    (F F' : function_context) (L L' : local_context) (ann : A) (τs1 τs2 : list type)
+    (le : local_effect) (es : expr A) :
+  F' = set fc_labels (cons (τs2, L')) F ->
+  L' = update_locals le L ->
+  expr_has_type F L es (ArrowT τs1 τs2) L' ->
+  instr_has_type F L (IBlock ann (ArrowT τs1 τs2) le es) (ArrowT τs1 τs2) L'
+| TLoop
+    (F F' : function_context) (L : local_context) (ann : A) (τs1 τs2 : list type) (es : expr A) :
+  F' = set fc_labels (cons (τs1, L)) F ->
+  expr_has_type F L es (ArrowT τs1 τs2) L ->
+  instr_has_type F L (ILoop ann (ArrowT τs1 τs2) es) (ArrowT τs1 τs2) L
+| TIte
+    (F : function_context) (L L' : local_context) (ann : A) (τa : arrow_type) (le : local_effect)
+    (es1 es2 : expr A) :
+  L' = update_locals le L ->
+  expr_has_type F L es1 τa L' ->
+  expr_has_type F L es2 τa L' ->
+  instr_has_type F L (IIte ann τa le es1 es2) τa L'
+| TBr
+    (F : function_context) (L L' : local_context) (ann : A) (n : nat) (τs τs1 τs2 : list type)
+    (le : local_effect) :
+  L' = update_locals le L ->
+  nth_error F.(fc_labels) n = Some (τs, L) ->
+  Forall (is_unrestricted F) τs1 ->
+  instr_has_type F L (IBr ann n) (ArrowT (τs1 ++ τs) τs2) L'
+| TBrIf (F : function_context) (L : local_context) (ann : A) (n : nat) (τs : list type) :
+  nth_error F.(fc_labels) n = Some (τs, L) ->
+  instr_has_type F L (IBrIf ann n) (ArrowT (τs ++ [NumT (IntT I32T)]) τs) L
+| TBrTable
+    (F : function_context) (L L' : local_context) (ann : A) (ns : list nat) (n : nat)
+    (τs τs1 τs2 : list type) :
+  Forall (fun i => nth_error F.(fc_labels) i = Some (τs, L)) (n :: ns) ->
+  Forall (is_unrestricted F) τs1 ->
+  instr_has_type F L (IBrTable ann ns n) (ArrowT (τs1 ++ τs ++ [NumT (IntT I32T)]) τs2) L'
+| TReturn
+    (F : function_context) (L L' : local_context) (ann : A) (le : local_effect)
+    (τs τs1 τs2 : list type) :
+  F.(fc_result_type) = τs ->
+  L' = update_locals le L ->
+  Forall (is_unrestricted F) τs1 ->
+  instr_has_type F L (IReturn ann) (ArrowT (τs1 ++ τs) τs2) L'
+
+with expr_has_type {A : Type} :
+  function_context -> local_context -> expr A -> arrow_type -> local_context -> Prop :=
+| TNil (F : function_context) (L : local_context) :
+  expr_has_type F L [] (ArrowT [] []) L
+| TCons
+    (F : function_context) (L1 L2 L3 : local_context) (e : instr A) (es : expr A)
+    (τs1 τs2 τs3 : list type) :
+  instr_has_type F L1 e (ArrowT τs1 τs2) L2 ->
+  expr_has_type F L2 es (ArrowT τs2 τs3) L3 ->
+  expr_has_type F L1 (e :: es) (ArrowT τs1 τs3) L3.
